refining reduction lemma in refl

examples/dsls/mini_steel/Pulse.Soundness.Return.fsti
@@ -7,42 +7,40 @@ open Pulse.Elaborate.Core
 open Pulse.Typing
 open Pulse.Soundness.Common
 
+module R = FStar.Reflection
 module EPure = Pulse.Elaborate.Pure
 module RT = Refl.Typing
 
-
-let return_post_with_eq (u:universe) (a:term) (x:term) (p:term) : term =
+let return_post_with_eq (u:universe) (a:term) (e:term) (p:term) (x:var) : term =
+  let x_tm = var_as_term x in
   let eq2_tm =
     let t = pack_ln (Tv_UInst (pack_fv (mk_steel_wrapper_lid "eq2_prop")) [u]) in
     let t = pack_ln (Tv_App t (a, Q_Implicit)) in
-    let t = pack_ln (Tv_App t (bound_var 0, Q_Explicit)) in
-    pack_ln (Tv_App t (x, Q_Explicit)) in
+    let t = pack_ln (Tv_App t (x_tm, Q_Explicit)) in
+    pack_ln (Tv_App t (e, Q_Explicit)) in
 
-  let p_app_0 = pack_ln (Tv_App p (bound_var 0, Q_Explicit)) in
+  let p_app_x = pack_ln (Tv_App p (x_tm, Q_Explicit)) in
   
-  let star_tm =
-    let t = pack_ln (Tv_FVar (pack_fv star_lid)) in
-    let t = pack_ln (Tv_App t (p_app_0, Q_Explicit)) in
-    pack_ln (Tv_App t (eq2_tm, Q_Explicit)) in
+  let star_tm = mk_star p_app_x eq2_tm in
 
-  mk_abs a Q_Explicit star_tm
+  mk_abs a Q_Explicit (RT.open_or_close_term' star_tm (RT.CloseVar x) 0)
 
 val return_stt_typing
-  (#f:stt_env)
-  (#g:env)
+  (#g:R.env)
   (#u:universe)
   (#a:term)
-  (#x:term)
+  (#e:term)
   (#p:term)
-  (a_typing:RT.typing (extend_env_l f g) a (pack_ln (Tv_Type u)))
-  (x_typing:RT.typing (extend_env_l f g) x a)
-  (p_typing:RT.typing (extend_env_l f g) p (mk_arrow (a, Q_Explicit) vprop_tm))
+  (x:var{None? (RT.lookup_bvar g x)})
+  (a_typing:RT.typing g a (pack_ln (Tv_Type u)))
+  (e_typing:RT.typing g e a)
+  (p_typing:RT.typing g p (mk_arrow (a, Q_Explicit) vprop_tm))
 
-  : GTot (RT.typing (extend_env_l f g)
-                    (mk_stt_return u a x p)
+  : GTot (RT.typing g
+                    (mk_stt_return u a e p)
                     (mk_stt_comp u a
-                       (pack_ln (Tv_App p (x, Q_Explicit)))
-                       (return_post_with_eq u a x p)))
+                       (pack_ln (Tv_App p (e, Q_Explicit)))
+                       (return_post_with_eq u a e p x)))
 
 val return_stt_noeq_typing
   (#f:stt_env)
@@ -60,21 +58,21 @@ val return_stt_noeq_typing
                     (mk_stt_comp u a (pack_ln (Tv_App p (x, Q_Explicit))) p))
 
 val return_stt_atomic_typing
-  (#f:stt_env)
-  (#g:env)
+  (#g:R.env)
   (#u:universe)
   (#a:term)
-  (#x:term)
+  (#e:term)
   (#p:term)
-  (a_typing:RT.typing (extend_env_l f g) a (pack_ln (Tv_Type u)))
-  (x_typing:RT.typing (extend_env_l f g) x a)
-  (p_typing:RT.typing (extend_env_l f g) p (mk_arrow (a, Q_Explicit) vprop_tm))
+  (x:var{None? (RT.lookup_bvar g x)})
+  (a_typing:RT.typing g a (pack_ln (Tv_Type u)))
+  (e_typing:RT.typing g e a)
+  (p_typing:RT.typing g p (mk_arrow (a, Q_Explicit) vprop_tm))
 
-  : GTot (RT.typing (extend_env_l f g)
-                    (mk_stt_atomic_return u a x p)
+  : GTot (RT.typing g
+                    (mk_stt_atomic_return u a e p)
                     (mk_stt_atomic_comp u a emp_inames_tm
-                       (pack_ln (Tv_App p (x, Q_Explicit)))
-                       (return_post_with_eq u a x p)))
+                       (pack_ln (Tv_App p (e, Q_Explicit)))
+                       (return_post_with_eq u a e p x)))
 
 val return_stt_atomic_noeq_typing
   (#f:stt_env)
@@ -92,21 +90,21 @@ val return_stt_atomic_noeq_typing
                     (mk_stt_atomic_comp u a emp_inames_tm (pack_ln (Tv_App p (x, Q_Explicit))) p))
 
 val return_stt_ghost_typing
-  (#f:stt_env)
-  (#g:env)
+  (#g:R.env)
   (#u:universe)
   (#a:term)
-  (#x:term)
+  (#e:term)
   (#p:term)
-  (a_typing:RT.typing (extend_env_l f g) a (pack_ln (Tv_Type u)))
-  (x_typing:RT.typing (extend_env_l f g) x a)
-  (p_typing:RT.typing (extend_env_l f g) p (mk_arrow (a, Q_Explicit) vprop_tm))
+  (x:var{None? (RT.lookup_bvar g x)})
+  (a_typing:RT.typing g a (pack_ln (Tv_Type u)))
+  (e_typing:RT.typing g e a)
+  (p_typing:RT.typing g p (mk_arrow (a, Q_Explicit) vprop_tm))
 
-  : GTot (RT.typing (extend_env_l f g)
-                    (mk_stt_ghost_return u a x p)
+  : GTot (RT.typing g
+                    (mk_stt_ghost_return u a e p)
                     (mk_stt_ghost_comp u a emp_inames_tm
-                       (pack_ln (Tv_App p (x, Q_Explicit)))
-                       (return_post_with_eq u a x p)))
+                       (pack_ln (Tv_App p (e, Q_Explicit)))
+                       (return_post_with_eq u a e p x)))
 
 val return_stt_ghost_noeq_typing
   (#f:stt_env)
