examples/dsls/core/Refl.Typing.fsti
@@ -1217,9 +1217,6 @@ val beta_reduction (t:R.typ) (q:R.aqualv) (e:R.term) (arg:R.term)
   : Lemma (open_or_close_term' e (OpenWith arg) 0 ==
            R.pack_ln (R.Tv_App (mk_abs t q e) (arg, q)))
 
-val beta_reduction_bv0 (t:R.typ) (q:R.aqualv) (e:R.term)
-  : Lemma (R.pack_ln (R.Tv_App (mk_abs t q e) (bound_var 0, q)) == e)
-
 //
 // Type of the top-level tactic that would splice-in the definitions
 //
